Represent closed terms explicitly

ctx-equiv-ixfree/lang.v
@@ -1,7 +1,7 @@
 
 From CtxEquivIris Require Import persistent_pred.
 
-Require Import IxFree.Lib IxFree.Nat.
+From IxFree Require Import Lib Nat.
 
 (* From iris.prelude Require Import options.
 From iris.base_logic Require Import invariants bi algebra.
@@ -101,15 +101,15 @@ Inductive base_step : expr → expr → Prop :=
      base_step (Plus e1 e2) (eint n3) *)
   .
 
-Inductive evctx :=
+Inductive ectx :=
   | HoleCtx
-  | AppLCtx (K: evctx) (v2 : val)
-  | AppRCtx (e1 : expr) (K: evctx)
-  | PlusLCtx (K: evctx) (v2 : val)
-  | PlusRCtx (e1 : expr) (K: evctx)
+  | AppLCtx (K: ectx) (v2 : val)
+  | AppRCtx (e1 : expr) (K: ectx)
+  | PlusLCtx (K: ectx) (v2 : val)
+  | PlusRCtx (e1 : expr) (K: ectx)
   .
 
-Fixpoint fill (K : evctx) (e : expr) : expr :=
+Fixpoint fill (K : ectx) (e : expr) : expr :=
   match K with
   | HoleCtx => e
   | AppLCtx K v2 => app (fill K e) (of_val v2)
@@ -119,7 +119,7 @@ Fixpoint fill (K : evctx) (e : expr) : expr :=
   end.
 
 (* filling a context with another context *)
-Fixpoint comp_ectx (Ko Ki: evctx) :=
+Fixpoint comp_ectx (Ko Ki: ectx) :=
   match Ko with
   | HoleCtx => Ki
   | AppLCtx K v2 => AppLCtx (comp_ectx K Ki) v2
@@ -151,12 +151,14 @@ Definition obs_eqv e1 e2 :=
 Infix "≈" := equiterminate (at level 80, right associativity, only printing).
 Infix "≡obs" := obs_eqv (at level 80, right associativity, only printing).
 
+
+
 (* Section logrel.
 Context `{heapGS Σ}.
 
 (* Definition valO := leibnizO val.
 Definition exprO := leibnizO expr.
-Definition evctxO := leibnizO evctx. *)
+Definition evctxO := leibnizO ectx. *)
 
 (* Definition val_rel := valO -n> valO -n> iProp Σ.
 Definition ctx_rel := evctxO -n> evctxO -n> iProp Σ.
@@ -164,11 +166,11 @@ Definition expr_rel := exprO -n> exprO -n> iProp Σ. *)
 
 Definition val_rel := persistent_pred (val * val) (iPropI Σ).
 Definition expr_rel := persistent_pred (expr * expr) (iPropI Σ).
-Definition evctx_rel := persistent_pred (evctx * evctx) (iPropI Σ).
+Definition evctx_rel := persistent_pred (ectx * ectx) (iPropI Σ).
 
 Definition val_relO := persistent_predO (val * val) (iPropI Σ).
 Definition expr_relO := persistent_predO (expr * expr) (iPropI Σ).
-Definition evctx_relO := persistent_predO (evctx * evctx) (iPropI Σ).
+Definition evctx_relO := persistent_predO (ectx * ectx) (iPropI Σ).
 
 Definition mk_val_rel (pred : (val * val) → iProp Σ) {Pers : ∀ v, Persistent (pred v)} : val_rel :=
   @PersPred _ _ pred Pers.
@@ -178,7 +180,7 @@ Definition mk_expr_rel (pred : (expr * expr) → iProp Σ) {Pers : ∀ e, Persis
   @PersPred _ _ pred Pers.
 Global Instance expr_rel_pers (τ : expr_relO) : ∀ e, Persistent (τ e) := _.
 
-Definition mk_evctx_rel (pred : (evctx * evctx) → iProp Σ) {Pers : ∀ E, Persistent (pred E)} : evctx_rel :=
+Definition mk_evctx_rel (pred : (ectx * ectx) → iProp Σ) {Pers : ∀ E, Persistent (pred E)} : evctx_rel :=
   @PersPred _ _ pred Pers.
 Global Instance evctx_rel_pers (τ : evctx_relO) : ∀ E, Persistent (τ E) := _.
 
@@ -187,53 +189,8 @@ Global Instance evctx_rel_pers (τ : evctx_relO) : ∀ E, Persistent (τ E) := _
 (* Locate "<pers>". *)
 
 (* Definition semtypeO := persistent_predO val (iPropI Σ). *)
+*)
 
-Definition L_rel_pre (L_rel:expr_rel) : expr_rel :=
-  mk_expr_rel (fun e =>
-    ((∀ v1, ⌜to_val e.1 = Some v1⌝ → ⌜terminates e.2⌝) ∗
-      (∀ e1', ⌜base_step e.1 e1'⌝ → ▷ L_rel (e1', e.2)))%I).
-
-Definition O_rel_pre (L_rel:expr_rel) : expr_rel :=
-  mk_expr_rel (fun e =>
-    (L_rel (e.1, e.2) ∧ L_rel (e.2, e.1))%I).
-
-Instance L_rel_pre_contractive :
-  Contractive L_rel_pre.
-Proof. solve_contractive. Qed.
-
-Definition L_rel : expr_rel := fixpoint L_rel_pre.
-Definition O_rel : expr_rel := O_rel_pre L_rel.
-
-Definition K_rel_pre (V_rel:val_rel) : evctx_rel :=
-  mk_evctx_rel (fun E =>
-    ∀ (v1 v2:val), □ (V_rel (v1, v2) →
-      O_rel (fill E.1 (of_val v1), fill E.2 (of_val v2))))%I.
-
-Definition R_rel_pre (V_rel:val_rel) : expr_rel :=
-  mk_expr_rel (fun e =>
-    ∀ (E1 E2:evctx), □ (▷ K_rel_pre V_rel (E1, E2) →
-      O_rel (fill E1 e.1, fill E2 e.2)))%I.
-
-Definition V_rel_pre (V_rel:val_rel) : val_rel :=
-  mk_val_rel (fun v =>
-    ∀ (v1' v2':val), □ (▷ V_rel (v1', v2') →
-      R_rel_pre V_rel (app (of_val v.1) (of_val v1'),
-        app (of_val v.2) (of_val v2'))))%I.
-
-Instance V_rel_pre_contractive :
-  Contractive (V_rel_pre).
-Proof. solve_contractive. Qed.
-
-Definition V_rel : val_rel := fixpoint V_rel_pre.
-Definition K_rel : evctx_rel := K_rel_pre V_rel.
-Definition R_rel : expr_rel := R_rel_pre V_rel.
-
-Definition E_rel : expr_rel :=
-  mk_expr_rel (fun e =>
-    ∀ (E1 E2:evctx), □ (K_rel (E1, E2) →
-      O_rel (fill E1 e.1, fill E2 e.2)))%I.
-
-(* open relations *)
 
 Definition sub := gmap string val.
 
@@ -253,6 +210,388 @@ with subst_map (xs : sub) (e : expr) : expr :=
   (* | abs x e => abs x (subst_map (binder_delete x xs) e) *)
   | eplus e1 e2 => eplus (subst_map xs e1) (subst_map xs e2)
   end.
+
+Fixpoint is_closed (X : list string) (e : expr) : bool :=
+  match e with
+  | var x => bool_decide (x ∈ X)
+  | evalue vunit | evalue (vint _) => true
+  | evalue (vlambda x e) => is_closed (x :b: X) e
+  | app e1 e2 | eplus e1 e2 => is_closed X e1 && is_closed X e2
+  end.
+Definition closed (X : list string) (e : expr) : Prop := Is_true (is_closed X e).
+
+(* Record cexpr := mk_cexpr {
+  cexpr_car :> expr;
+  cexpr_closed : is_closed [] cexpr_car;
+}.
+
+Record cval := mk_cval {
+  cval_car :> val;
+  cval_closed : is_closed [] cval_car;
+}.
+
+Definition cval_to_cexpr (v:cval) : cexpr :=
+  mk_cexpr (cval_car v) (cval_closed v).
+
+Coercion cval_to_cexpr : cval >-> cexpr. *)
+
+(* Definition cexpr_rel := cexpr ⇒ᵢ cexpr ⇒ᵢ IRel.
+Definition cval_rel := cval ⇒ᵢ cval ⇒ᵢ IRel. *)
+
+(* Definition cexpr_rel := .
+Record cexpr_rel := mk_cexpr_rel {
+  cexpr_rel_car :> expr ⇒ᵢ expr ⇒ᵢ IRel;
+  cexpr_rel_closed e1 e2 : cexpr_rel_car e1 e2 → is_closed [] e1 ∧ is_closed [] e2;
+}. *)
+
+Definition expr_rel := expr ⇒ᵢ expr ⇒ᵢ IRel.
+Definition val_rel := val ⇒ᵢ val ⇒ᵢ IRel.
+Definition sub_rel := sub ⇒ᵢ sub ⇒ᵢ IRel.
+Definition ctx_rel := ectx ⇒ᵢ ectx ⇒ᵢ IRel.
+(* Definition Obs_sig := expr ⇒ᵢ expr ⇒ᵢ IRel. *)
+
+Definition L_rel_pre (L_rel:expr_rel) : expr_rel :=
+  λ e1 e2,
+    (closed [] e1)ᵢ →ᵢ (closed [] e2)ᵢ →ᵢ
+    (∀ v1 : val, e1 = v1 → terminates e2)ᵢ ∧ᵢ
+    ∀ᵢ e1' : expr, (base_step e1 e1')ᵢ →ᵢ ▷ L_rel e1' e2.
+
+Lemma L_rel_pre_contractive : contractive L_rel_pre.
+Proof.
+  intro n; iintros; unfold L_rel_pre; auto_contr.
+Qed.
+
+Definition L_rel_fix := I_fix L_rel_pre.
+Definition L_rel := L_rel_pre L_rel_fix.
+(* Definition L_rel := I_fix L_rel_pre. *)
+
+Definition O_rel e₁ e₂ := L_rel e₁ e₂ ∧ᵢ L_rel e₂ e₁.
+
+(* ========================================================================= *)
+
+Lemma L_rel_roll p₁ p₂ n :
+  n ⊨ L_rel p₁ p₂ → n ⊨ L_rel_fix p₁ p₂.
+Proof.
+  intro H; iapply (I_fix_roll expr_rel); [ | exact H ].
+  apply L_rel_pre_contractive.
+Qed.
+
+Lemma L_rel_unroll p₁ p₂ n :
+  n ⊨ L_rel_fix p₁ p₂ → n ⊨ L_rel p₁ p₂.
+Proof.
+  intro H; iapply (I_fix_unroll expr_rel); [ | exact H ].
+  apply L_rel_pre_contractive.
+Qed.
+
+Definition K_rel_pre (V_rel : val_rel) (E₁ E₂ : ectx) :=
+  ∀ᵢ v1 v2 : val,
+    (closed [] v1)ᵢ →ᵢ (closed [] v2)ᵢ →ᵢ
+    V_rel v1 v2 →ᵢ O_rel (fill E₁ v1) (fill E₂ v2).
+
+Definition R_rel_pre (V_rel : val_rel) (e₁ e₂ : expr) :=
+  ∀ᵢ E₁ E₂, ▷ K_rel_pre V_rel E₁ E₂ →ᵢ O_rel (fill E₁ e₁) (fill E₂ e₂).
+
+Definition V_rel_pre (V_rel : val_rel) : val_rel :=
+  λ v1 v2, (closed [] v1)ᵢ →ᵢ (closed [] v2)ᵢ →ᵢ
+  ∀ᵢ (u1 u2:val), (closed [] u1)ᵢ →ᵢ (closed [] u2)ᵢ →ᵢ
+    ▷ V_rel u1 u2 →ᵢ R_rel_pre V_rel (app v1 u1) (app v2 u2).
+
+Definition V_rel_fix := I_fix V_rel_pre.
+
+Definition V_rel := V_rel_pre V_rel_fix.
+Definition R_rel := R_rel_pre V_rel_fix.
+Definition K_rel := K_rel_pre V_rel_fix.
+
+Definition E_rel (e1 e2 : expr) : IProp :=
+  (closed [] e1)ᵢ →ᵢ (closed [] e2)ᵢ →ᵢ
+  ∀ᵢ E1 E2 : ectx, K_rel E1 E2 →ᵢ
+    O_rel (fill E1 e1) (fill E2 e2).
+
+(* ========================================================================= *)
+(* Open relations *)
+
+Definition G_rel (γ1 γ2 : sub) : IProp :=
+  ∀ᵢ x v1 v2,
+    (γ1 !! x = Some v1)ᵢ →ᵢ
+    (γ2 !! x = Some v2)ᵢ →ᵢ
+    V_rel v1 v2.
+
+Definition E_rel_o (e₁ e₂ : expr) : IProp :=
+  ∀ᵢ γ₁ γ₂, G_rel γ₁ γ₂ →ᵢ E_rel (subst_map γ₁ e₁) (subst_map γ₂ e₂).
+
+Definition V_rel_o (v₁ v₂ : val) : IProp :=
+  ∀ᵢ γ₁ γ₂, G_rel γ₁ γ₂ →ᵢ V_rel (subst_map_val γ₁ v₁) (subst_map_val γ₂ v₂).
+
+(* Definition rel_p (p₁ p₂ : expr) : IProp :=
+  ∀ᵢ γ₁ γ₂, G_rel γ₁ γ₂ →ᵢ O_rel (bind γ₁ p₁) (bind γ₂ p₂). *)
+
+(* ========================================================================= *)
+(* Contractiveness and urolling fixpoint *)
+
+Lemma V_rel_pre_contractive : contractive V_rel_pre.
+Proof.
+  intro n; iintros; unfold V_rel_pre, R_rel_pre, K_rel_pre; auto_contr.
+Qed.
+
+Lemma V_rel_roll v₁ v₂ n :
+  n ⊨ V_rel v₁ v₂ → n ⊨ V_rel_fix v₁ v₂.
+Proof.
+  intro H; iapply (I_fix_roll val_rel); [ | exact H ].
+  apply V_rel_pre_contractive.
+Qed.
+
+Lemma V_rel_unroll v₁ v₂ n :
+  n ⊨ V_rel_fix v₁ v₂ → n ⊨ V_rel v₁ v₂.
+Proof.
+  intro H; iapply (I_fix_unroll val_rel); [ | exact H ].
+  apply V_rel_pre_contractive.
+Qed.
+
+Lemma V_rel_intro (v1 v2 : val) n :
+  n ⊨ ((closed [] v1)ᵢ →ᵢ (closed [] v2)ᵢ →ᵢ ∀ᵢ (u1 u2:val),
+    (closed [] u1)ᵢ →ᵢ (closed [] u2)ᵢ →ᵢ
+    ▷ V_rel u1 u2 →ᵢ R_rel (app v1 u1) (app v2 u2)) →
+  n ⊨ V_rel v1 v2.
+Proof.
+  intros Hv.
+  iintros Hcv1 Hcv2 u1 u2 Hcu1 Hcu2 Hl.
+  iapply Hv; auto.
+  later_shift. apply V_rel_unroll; assumption.
+Qed.
+
+Lemma V_rel_elim (v1 v2 u1 u2 : val) n :
+  n ⊨ V_rel v1 v2 →
+  n ⊨ (closed [] v1)ᵢ →
+  n ⊨ (closed [] v2)ᵢ →
+  n ⊨ (closed [] u1)ᵢ →
+  n ⊨ (closed [] u2)ᵢ →
+  n ⊨ ▷ V_rel u1 u2 →
+  n ⊨ R_rel (app v1 u1) (app v2 u2).
+Proof.
+  intros Hv Hcv1 Hcv2 Hcu1 Hcu2 Hu.
+  iapply Hv; auto.
+  later_shift. apply V_rel_roll. assumption.
+Qed.
+
+Lemma K_rel_intro (E₁ E₂ : ectx) n :
+  n ⊨ (∀ᵢ (v₁ v₂:val), (closed [] v₁)ᵢ →ᵢ (closed [] v₂)ᵢ →ᵢ
+    V_rel v₁ v₂ →ᵢ O_rel (fill E₁ v₁) (fill E₂ v₂)) →
+  n ⊨ K_rel E₁ E₂.
+Proof.
+  intro HE. iintros v₁ v₂ Hcv1 Hcv2 Hv. iapply HE; auto.
+  apply V_rel_unroll; assumption.
+Qed.
+
+Lemma K_rel_elim (E₁ E₂ : ectx) (v₁ v₂ : val) n :
+  n ⊨ K_rel E₁ E₂ →
+  n ⊨ (closed [] v₁)ᵢ →
+  n ⊨ (closed [] v₂)ᵢ →
+  n ⊨ V_rel v₁ v₂ →
+  n ⊨ O_rel (fill E₁ v₁) (fill E₂ v₂).
+Proof.
+  intros HE Hc1 Hc2 Hv. iapply HE; auto. apply V_rel_roll; assumption.
+Qed.
+
+Lemma R_rel_elim (e₁ e₂ : expr) E₁ E₂ n :
+  n ⊨ R_rel e₁ e₂ →
+  n ⊨ ▷ K_rel E₁ E₂ →
+  n ⊨ O_rel (fill E₁ e₁) (fill E₂ e₂).
+Proof.
+  intros He HE; iapply He; assumption.
+Qed.
+
+Lemma E_rel_elim (e₁ e₂ : expr) E₁ E₂ n :
+  n ⊨ E_rel e₁ e₂ →
+  n ⊨ (closed [] e₁)ᵢ →
+  n ⊨ (closed [] e₂)ᵢ →
+  n ⊨ K_rel E₁ E₂ →
+  n ⊨ O_rel (fill E₁ e₁) (fill E₂ e₂).
+Proof.
+  intros He Hc1 Hc2 HE. iapply He; auto.
+Qed.
+
+Lemma V_rel_elimE (v1 v2 u1 u2 : val) n :
+  n ⊨ V_rel v1 v2 →
+  n ⊨ (closed [] v1)ᵢ →
+  n ⊨ (closed [] v2)ᵢ →
+  n ⊨ (closed [] u1)ᵢ →
+  n ⊨ (closed [] u2)ᵢ →
+  n ⊨ V_rel u1 u2 →
+  n ⊨ E_rel (app v1 u1) (app v2 u2).
+Proof.
+  intros Hv Hcv1 Hcv2 Hcu1 Hcu2 Hu. iintros Hc1 Hc2 E₁ E₂ HE.
+  (* idestruct Hc1. *)
+  (* idestruct Hc2. *)
+  apply R_rel_elim. 2: { later_shift; assumption. }
+  apply V_rel_elim; auto.
+  later_shift; assumption.
+Qed.
+
+Lemma compat_val (v₁ v₂ : val) n :
+  n ⊨ V_rel_o v₁ v₂ →
+  n ⊨ E_rel_o v₁ v₂.
+Proof.
+  intro Hv. iintros γ₁ γ₂ Hγ Hc1 Hc2 E₁ E₂. iintros HE. simpl.
+  apply K_rel_elim; auto.
+  iapply Hv. assumption.
+Qed.
+
+Lemma compat_app (e₁ e₂ e₁' e₂' : expr) n :
+  n ⊨ E_rel_o e₁ e₂ →
+  n ⊨ E_rel_o e₁' e₂' →
+  n ⊨ E_rel_o (app e₁ e₁') (app e₂ e₂').
+Proof.
+  intros He He'.
+  iintros γ₁ γ₂ Hγ E₁ E₂ HE.
+  (* term_simpl. *)
+  (* Check E_rel_intro. *)
+  pose proof E_rel_elim.
+  (* apply E_rel_elim. *)
+  (* apply (E_rel_elim _ _ (AppRCtx _ _) (AppRCtx _ _)). *)
+  (* eapply (E_rel_elim _ _ (AppLCtx _ _) (AppLCtx _ _)). *)
+  (* eapply E_rel_elim with (E₁ := AppRCtx _ _) (E₂ := AppRCtx _ _). *)
+    (* [ *)
+     - simpl.
+
+     Print K_rel_pre.
+     iapply He. assumption.
+      (* | ]. *)
+  apply K_rel_intro; iintros v₁ v₂ Hv.
+  apply E_rel_elim with (E₁ := ectx_app2 _ _) (E₂ := ectx_app2 _ _);
+    [ iapply He'; assumption | ].
+  apply K_rel_intro; iintros u₁ u₂ Hu; simpl.
+  iapply V_rel_elimE; assumption.
+Qed.
+
+(* Lemma rel_e_compat_callcc {V : Set} (e₁ e₂ : expr (inc V)) n :
+  n ⊨ E_rel e₁ e₂ →
+  n ⊨ E_rel (e_callcc e₁) (e_callcc e₂).
+Proof.
+  intro He.
+  iintros γ₁ γ₂ Hγ E₁ E₂ HE; term_simpl.
+  eapply Obs_red_both; [ auto_red | auto_red | ]; later_shift.
+  unfold subst; repeat rewrite bind_bind_comp'.
+  iapply He; [ | eassumption ].
+  iintro x; destruct x as [ | x ]; term_simpl; [ | iapply Hγ ].
+  apply V_rel_intro; iintros u₁ u₂ Hu F₁ F₂ HF.
+  eapply Obs_red_both; [ auto_red | auto_red | ]; later_shift; term_simpl.
+  eapply Obs_red_both; [ auto_red | auto_red | ]; later_shift; term_simpl.
+  apply K_rel_elim; assumption.
+Qed.
+
+Lemma rel_e_compat_abort {V : Set} (p₁ p₂ : program V) n :
+  n ⊨ rel_p p₁ p₂ →
+  n ⊨ E_rel (e_abort p₁) (e_abort p₂).
+Proof.
+  intro Hp.
+  iintros γ₁ γ₂ Hγ E₁ E₂ HE; term_simpl.
+  eapply Obs_red_both; [ auto_red | auto_red | ]; later_shift; term_simpl.
+  iapply Hp; assumption.
+Qed. *)
+
+
+Lemma rel_v_compat_var {V : Set} (x : V) n :
+  n ⊨ rel_v (v_var x) (v_var x).
+Proof.
+  iintros γ₁ γ₂ Hγ; iapply Hγ.
+Qed.
+
+Lemma rel_v_compat_lam {V : Set} (e₁ e₂ : expr (inc V)) n :
+  n ⊨ E_rel e₁ e₂ →
+  n ⊨ rel_v (v_lam e₁) (v_lam e₂).
+Proof.
+  intro He;
+  iintros γ₁ γ₂ Hγ; term_simpl.
+  apply V_rel_intro; iintros u₁ u₂ Hu.
+  eapply R_rel_red_both; [ auto_red | auto_red | ]; later_shift; term_simpl.
+  unfold subst; repeat rewrite bind_bind_comp'.
+  iapply He.
+  iintro x; destruct x as [ | x ]; term_simpl.
+  + assumption.
+  + iapply Hγ.
+Qed.
+
+(* ========================================================================= *)
+(* programs *)
+
+Lemma rel_p_compat_expr {V : Set} (e₁ e₂ : expr V) n :
+  n ⊨ E_rel e₁ e₂ →
+  n ⊨ rel_p e₁ e₂.
+Proof.
+  intro He.
+  iintros γ₁ γ₂ Hγ; term_simpl.
+  apply E_rel_elim with (E₁ := ectx_hole) (E₂ := ectx_hole).
+  + iapply He; assumption.
+  + apply K_rel_intro; iintros v₁ v₂ Hv; apply Obs_value.
+Qed.
+
+Fixpoint fundamental_property_e {V : Set} (e : expr V) n :
+  n ⊨ E_rel e e
+with fundamental_property_v {V : Set} (v : value V) n :
+  n ⊨ rel_v v v
+with fundamental_property_p {V : Set} (p : program V) n :
+  n ⊨ rel_p p p.
+Proof.
++ destruct e.
+  - apply rel_e_compat_value, fundamental_property_v.
+  - apply compat_app; apply fundamental_property_e.
+  - apply rel_e_compat_callcc, fundamental_property_e.
+  -  apply rel_e_compat_abort, fundamental_property_p.
++ destruct v.
+  - apply rel_v_compat_var.
+  - apply rel_v_compat_lam, fundamental_property_e.
++ destruct p.
+  - apply rel_p_compat_expr, fundamental_property_e.
+Qed.
+
+(* Definition F_ObsL (ObsL : Obs_sig) : Obs_sig :=
+  λ p₁ p₂,
+  (∀ v₁ : val, p₁ = v₁ → terminates p₂)ᵢ ∧ᵢ
+  ∀ᵢ p₁' : program ∅, (red p₁ p₁')ᵢ →ᵢ ▷ ObsL p₁' p₂. *)
+
+(*
+
+Definition O_rel_pre (L_rel:expr_rel) : expr_rel :=
+  mk_expr_rel (fun e =>
+    (L_rel (e.1, e.2) ∧ L_rel (e.2, e.1))%I).
+
+Instance L_rel_pre_contractive :
+  Contractive L_rel_pre.
+Proof. solve_contractive. Qed.
+
+Definition L_rel : expr_rel := fixpoint L_rel_pre.
+Definition O_rel : expr_rel := O_rel_pre L_rel.
+
+Definition K_rel_pre (V_rel:val_rel) : evctx_rel :=
+  mk_evctx_rel (fun E =>
+    ∀ (v1 v2:val), □ (V_rel (v1, v2) →
+      O_rel (fill E.1 (of_val v1), fill E.2 (of_val v2))))%I.
+
+Definition R_rel_pre (V_rel:val_rel) : expr_rel :=
+  mk_expr_rel (fun e =>
+    ∀ (E1 E2:ectx), □ (▷ K_rel_pre V_rel (E1, E2) →
+      O_rel (fill E1 e.1, fill E2 e.2)))%I.
+
+Definition V_rel_pre (V_rel:val_rel) : val_rel :=
+  mk_val_rel (fun v =>
+    ∀ (v1' v2':val), □ (▷ V_rel (v1', v2') →
+      R_rel_pre V_rel (app (of_val v.1) (of_val v1'),
+        app (of_val v.2) (of_val v2'))))%I.
+
+Instance V_rel_pre_contractive :
+  Contractive (V_rel_pre).
+Proof. solve_contractive. Qed.
+
+Definition V_rel : val_rel := fixpoint V_rel_pre.
+Definition K_rel : evctx_rel := K_rel_pre V_rel.
+Definition R_rel : expr_rel := R_rel_pre V_rel.
+
+Definition E_rel : expr_rel :=
+  mk_expr_rel (fun e =>
+    ∀ (E1 E2:ectx), □ (K_rel (E1, E2) →
+      O_rel (fill E1 e.1, fill E2 e.2)))%I.
+
+(* open relations *)
 
 (* Definition subO := leibnizO sub. *)
 (* Definition sub_rel := subO -n> subO -n> iProp Σ. *)
@@ -308,7 +647,7 @@ Lemma erel_to_vrel e1 e2 v1 v2:
 Proof.
 Admitted.
 
-Lemma RelK_elim (E1 E2 : evctx) (v1 v2 : val) :
+Lemma K_rel_elim (E1 E2 : ectx) (v1 v2 : val) :
   (⊢ K_rel (E1, E2)) →
   (⊢ V_rel (v1, v2)) →
   ⊢ O_rel (fill E1 (of_val v1), fill E2 (of_val v2)).
@@ -320,7 +659,7 @@ Proof.
   iApply Hv.
 Qed.
 
-Lemma RelK_elim1 (E1 E2 : evctx) (v1 v2 : val) :
+Lemma K_rel_elim1 (E1 E2 : ectx) (v1 v2 : val) :
   K_rel (E1, E2) ∧ V_rel (v1, v2)
   ⊢ O_rel (fill E1 (of_val v1), fill E2 (of_val v2)).
 Proof.
@@ -359,15 +698,15 @@ Proof.
 
   (* iApply "Hv". *)
 
-  (* Check RelK_elim1. *)
+  (* Check K_rel_elim1. *)
   (* iUnfold V_rel_o in "Hv". *)
 
-  (* iPoseProof (RelK_elim1 $! E1 E2 with "[HE]") as "H1". *)
+  (* iPoseProof (K_rel_elim1 $! E1 E2 with "[HE]") as "H1". *)
  (* g2 v1 v2 with "HE" *)
-  (* iAssert RelK_elim as "H1". *)
-  (* iSpecialize (RelK_elim). *)
+  (* iAssert K_rel_elim as "H1". *)
+  (* iSpecialize (K_rel_elim). *)
 
-  iApply RelK_elim1.
+  iApply K_rel_elim1.
   iSplit.
   - iApply "HK".
   -
